dijkstra/SpaceDijkGraph.v
@@ -7,11 +7,11 @@ Require Import CertiGraph.graph.AdjMatGraph.
 Local Open Scope logic.
 
 Lemma elabel_Znth_graph_to_mat:
-  forall (g: DijkGG) src dst,
+  forall inf size (g: (DijkGG inf size)) src dst,
     vvalid g src ->
     vvalid g dst ->
     elabel g (src, dst) =
-    Znth dst (Znth src (@graph_to_mat SIZE g id)).
+    Znth dst (Znth src (@graph_to_mat size g id)).
 Proof.
   intros.
   rewrite (vvalid_meaning g) in H, H0.
@@ -20,5 +20,4 @@ Proof.
   lia.
 Qed.
 
-Definition DijkGraph sh cs g gaddr : mpred := @SpaceAdjMatGraph SIZE sh cs id g gaddr.
-
+Definition DijkGraph sh cs g gaddr size : mpred := @SpaceAdjMatGraph size sh cs id g gaddr.
